mistrust.v
@@ -1,0 +1,34 @@
+Require Import Program.
+Require Import unSecureND.
+
+Lemma remove_empty: forall Pa f,
+  NDProof (profile_merge empty_profile Pa) f ->
+  NDProof Pa f.
+Proof.
+  intros. apply -> ndproof_m. apply H. reflexivity. rewrite profile_merge_empty_l. reflexivity.
+Qed.
+
+Ltac sprem :=
+  try assumption || (left; assumption) || (right; reflexivity) ||
+    (apply typable_impl; intro; apply typable_bottom) || apply empty_profile_typable.
+
+Lemma lemma1a: forall Ra Rb (* Pa Pb *) f1 f2 f3,
+  repository_lt Ra Rb -> (* typable_profile Ra Pa -> typable_profile Rb Pb -> *)
+  Resource.lt f1 f2 -> typable Ra f1 -> typable Ra f2 -> typable Rb f3 ->
+  NDProof (singleton_profile f1) (nd_impl (nd_read f3) nd_bottom) ->
+  NDProof (singleton_profile f2) (nd_impl (nd_read f3) nd_bottom).
+Proof.
+  intros.
+  apply nd_exec with Ra Rb; sprem.
+    apply singleton_profile_typable; assumption.
+  apply remove_empty.
+  apply nd_weakening with Ra Ra; sprem.
+  apply nd_write_intro with Ra Rb; sprem.
+  apply nd_read_intro with Ra Rb; sprem.
+  apply nd_trust_intro with Ra Rb; sprem.
+  apply nd_read_intro with Ra Rb; sprem.
+    simpl; trivial.
+  apply nd_trust_intro with Ra Ra; sprem.
+  apply nd_read_intro with Ra Rb; sprem.
+    simpl; trivial.
+Qed.
